Incomplete type preservation

theories/abs_imp.v
@@ -3,236 +3,681 @@ From ABS Require Import list_util abs_defs abs_util abs_functional_metatheory.
 
 (** * ABS Imperative Metatheory *)
 
+Notation id := nat.
+
 (* Imperative semantics based on FASE-20 paper – not generated from Ott, but probably should be *)
+Section Semantics.
+  Context
+      (Cs: list CL)
+      (Fs: list F)
+      (name_of: id -> f)
+      (id_of: f -> id)
+  .
 
-Equations get_class_name (CL0:CL): C := {get_class_name (class name _ _) := name}.
-Equations get_fields (CL0:CL): list (T*x) := {get_fields (class _ fields _) := fields}.
+  Equations get_class_name (CL0:CL): C := {get_class_name (class name _ _) := name}.
+  Equations get_fields (CL0:CL): list (T*x) := {get_fields (class _ fields _) := fields}.
+  Equations get_methods (CL0:CL): list M := {get_methods (class _ _ methods) := methods}.
 
-Notation queue := (gmultiset task).
+  Equations get_params (_:M): list (T*x) := {get_params (M_m _ _ params _ _ ) := params}.
+  Equations get_type (_:M): T := {get_type (M_m type _ _ _ _ ) := type}.
 
-Inductive cn: Type :=
-| cn_future (f0:f) (v:option t)
-| cn_object (C0:C) (a:s) (p:option task) (q: queue)
-| cn_invoc (o0:o) (f0:f) (m0:m) (vs: list t).
+  Definition queue := (gmultiset task).
 
-Notation config := (natmap cn).
-Definition add (p:task) (q:queue) := q ⊎ {[+ p +]}.
-Definition remove (p:task) (q:queue) := difference q {[+ p +]}.
+  Inductive cn: Type :=
+  | cn_future (f0:f) (v:option t)
+  | cn_object (C0:C) (a:s) (p:option task) (q: queue)
+  | cn_invoc (o0:o) (f0:f) (m0:m) (vs: list t).
 
-Equations get_method_decl (m0:m) (l: list M) : option M := {
-  get_method_decl _ [] := None ;
-  get_method_decl m ((M_m T m' params decl body)::Ms) :=
-      if String.eqb m m' then Some (M_m T m' params decl body) else get_method_decl m Ms
-  }.
+  Definition config := (natmap cn).
+  Definition add (p:task) (q:queue) := (q ⊎ {[+ p +]}).
+  Definition remove (p:task) (q:queue) := (q ∖ {[+ p +]}).
+  Equations get_method_decl (m0:m) (l: list M) : option M := {
+      get_method_decl _ [] := None ;
+      get_method_decl m ((M_m T m' params decl body)::Ms) :=
+        if String.eqb m m' then Some (M_m T m' params decl body) else get_method_decl m Ms
+    }.
 
-Equations bind_params_aux (s0:s) (vs: list t) (params: list (T*x)): s := {
-  bind_params_aux s0 [] _ := s0;
-  bind_params_aux s0 _ [] := s0;
-  bind_params_aux s0 (v::vs) ((_,x)::Txs) := insert x v (bind_params_aux s0 vs Txs)
-  }.
+  #[global] Instance elem_of_list_m: ElemOf m (list M) := fun m ms => get_method_decl m ms <> None.
 
-Definition bind_params := bind_params_aux empty.
+  Equations get_class_decl (c:C) (l: list CL) : option CL := {
+      get_class_decl _ [] := None ;
+      get_class_decl c ((class name fields methods)::Cs) :=
+        if String.eqb c name then Some (class name fields methods) else get_class_decl c Cs
+    }.
 
-Equations bind (m0:m) (vs: list t) (f0:f) (CL0:CL) : option task := {
-  bind m vs f (class n params m_list) :=
-  match get_method_decl m m_list with
-  | None => None
-  | Some (M_m T m' params decl body) =>
-      Some (tsk body (bind_params vs params))
-  end
-  }.
+  #[global] Instance elem_of_list_CL: ElemOf C (list CL) := fun c Cs => get_class_decl c Cs <> None.
 
-Definition reduce (Fs: list F): relation (e * s) :=
-  fun  x y => let (e0, s0) := x in let (e1, s1) := y in red_e Fs s0 e0 s1 e1.
-Definition eval (Fs: list F) (s0:s) (e0:e) (v:t): Prop :=
-  exists sf, (rtc (reduce Fs)) (e0, s0) (e_t v, sf).
+  Equations bind_params_aux (s0:s) (vs: list t) (params: list (T*x)): s := {
+      bind_params_aux s0 [] _ := s0;
+      bind_params_aux s0 _ [] := s0;
+      bind_params_aux s0 (v::vs) ((_,x)::Txs) := insert x v (bind_params_aux s0 vs Txs)
+    }.
 
-Equations eval_list (Fs: list F) (s0:s) (es: list e) (vs: list t): Prop := {
-    eval_list _ _ [] [] := True;
-    eval_list Fs s0 (e::es) (v::vs) := eval Fs s0 e v /\ eval_list Fs s0 es vs;
-    eval_list _ _ _ _ := False
-  }.
+  Definition bind_params := bind_params_aux empty.
 
-#[global]
-Instance elem_of_map: ElemOf x s := fun x s => s !! x <> None.
-#[global]
-Instance elem_of_config: ElemOf nat config := fun x s => s !! x <> None.
+  Equations bind (m0:m) (vs: list t) (f0:f) (CL0:CL) : option task := {
+      bind m vs f (class n params m_list) :=
+        match get_method_decl m m_list with
+        | None => None
+        | Some (M_m T m' params decl body) =>
+            Some (tsk body (bind_params vs params))
+        end
+    }.
 
-Definition destiny: f := "destiny"%string.
+  Definition eval (s0:s) (e0:e) (v:t): Prop :=
+    exists sf, (rtc (reduce Fs)) (e0, s0) (e_t v, sf).
 
-Inductive stmt_step (Fs:list F): list CL -> config -> config -> Prop :=
-| step_activate: forall Cs σ p q i a C,
-    p ∈ q ->
-    σ !! i = Some (cn_object C a None q) ->
-    stmt_step Fs Cs σ (<[i:=(cn_object C a (Some p) (remove p q))]> σ)
+  Equations eval_list (s0:s) (es: list e) (vs: list t): Prop := {
+      eval_list _ [] [] := True;
+      eval_list s0 (e::es) (v::vs) := eval s0 e v /\ eval_list s0 es vs;
+      eval_list _ _ _ := False
+    }.
 
-| step_asgn1: forall Cs σ i a C l x e s q v,
-    x ∈ l ->
-    eval Fs (union a l) e v ->
-    σ !! i = Some (cn_object C a (Some (tsk (stmt_seq (stmt_asgn x (rhs_e e)) s) l)) q) ->
-    stmt_step Fs Cs σ (<[i:=(cn_object C a (Some (tsk s (<[x:=v]> l))) q)]> σ)
+  Definition destiny: f := "destiny"%string.
 
-| step_asgn2: forall Cs σ o a C l x e s q v,
-    ~ x ∈ l ->
-    eval Fs (union a l) e v ->
-    σ !! o = Some (cn_object C a (Some (tsk (stmt_seq (stmt_asgn x (rhs_e e)) s) l)) q) ->
-    stmt_step Fs Cs σ (<[o:=(cn_object C (<[x:=v]> a) (Some (tsk s l)) q)]> σ)
+  Definition fresh (f0:f) (σ:config) : Prop := forall i f v, σ !! i = Some (cn_future f v) -> f <> f0.
 
-| step_cond1: forall Cs σ o a C l e s1 s2 s q,
-    eval Fs (union a l) e (t_b true) ->
-    σ !! o = Some (cn_object C a (Some (tsk (stmt_seq (stmt_cond e s1 s2) s) l)) q) ->
-    stmt_step Fs Cs σ (<[o:=cn_object C a (Some (tsk (stmt_seq s1 s) l)) q]> σ)
+  Inductive stmt_step: config -> config -> Prop :=
+  | step_activate: forall σ p q i a C,
+      p ∈ q ->
+      σ !! i = Some (cn_object C a None q) ->
+      stmt_step σ (<[i:=(cn_object C a (Some p) (remove p q))]> σ)
 
-| step_cond2: forall Cs σ o a C l e s1 s2 s q,
-    eval Fs (union a l) e (t_b false) ->
-    σ !! o = Some (cn_object C a (Some (tsk (stmt_seq (stmt_cond e s1 s2) s) l)) q) ->
-    stmt_step Fs Cs σ (<[o:=cn_object C a (Some (tsk (stmt_seq s2 s) l)) q]> σ)
+  | step_asgn1: forall σ i a C l x e s q v,
+      x ∈ dom l ->
+      eval (union a l) e v ->
+      σ !! i = Some (cn_object C a (Some (tsk (stmt_seq (stmt_asgn x (rhs_e e)) s) l)) q) ->
+      stmt_step σ (<[i:=(cn_object C a (Some (tsk s (<[x:=v]> l))) q)]> σ)
 
-| step_skip1: forall Cs σ o a C l s q,
-    σ !! o = Some (cn_object C a (Some (tsk (stmt_seq stmt_skip s) l)) q) ->
-    stmt_step Fs Cs σ (<[o:=cn_object C a (Some (tsk s l)) q]> σ)
+  | step_asgn2: forall σ o a C l x e s q v,
+      x ∈ dom a ->
+      eval (union a l) e v ->
+      σ !! o = Some (cn_object C a (Some (tsk (stmt_seq (stmt_asgn x (rhs_e e)) s) l)) q) ->
+      stmt_step σ (<[o:=(cn_object C (<[x:=v]> a) (Some (tsk s l)) q)]> σ)
 
-| step_skip2: forall Cs σ o a C l q,
-    σ !! o = Some (cn_object C a (Some (tsk stmt_skip l)) q) ->
-    stmt_step Fs Cs σ (<[o:=cn_object C a None q]> σ)
+  | step_cond1: forall σ o a C l e s1 s2 s q,
+      eval (union a l) e (t_b true) ->
+      σ !! o = Some (cn_object C a (Some (tsk (stmt_seq (stmt_cond e s1 s2) s) l)) q) ->
+      stmt_step σ (<[o:=cn_object C a (Some (tsk (stmt_seq s1 s) l)) q]> σ)
 
-| step_while: forall Cs σ o a C l e s1 s2 q,
-    σ !! o = Some (cn_object C a (Some (tsk (stmt_seq (stmt_loop e s1) s2) l)) q) ->
-    stmt_step Fs Cs σ (<[o:=cn_object C a (Some ( tsk (stmt_seq (stmt_cond e (stmt_seq s1 (stmt_loop e s1)) stmt_skip) s2) l)) q]> σ)
+  | step_cond2: forall σ o a C l e s1 s2 s q,
+      eval (union a l) e (t_b false) ->
+      σ !! o = Some (cn_object C a (Some (tsk (stmt_seq (stmt_cond e s1 s2) s) l)) q) ->
+      stmt_step σ (<[o:=cn_object C a (Some (tsk (stmt_seq s2 s) l)) q]> σ)
 
-| step_call: forall Cs σ oi o' a C l q x m es vs s f fi i,
-    ~ fi ∈ σ ->
-    ~ i ∈ σ ->
-    eval_list Fs (union a l) es vs ->
-    σ !! oi = Some (cn_object C a (Some (tsk (stmt_seq (stmt_asgn x (rhs_invoc o' m es)) s) l)) q) ->
-    stmt_step Fs Cs σ (<[oi:=cn_object C a (Some (tsk (stmt_seq (stmt_asgn x (rhs_get f)) s) l)) q]>
-                      (<[i:=cn_invoc o' f m vs]>
-                         (<[fi:=cn_future f None]> σ)))
+  | step_skip1: forall σ o a C l s q,
+      σ !! o = Some (cn_object C a (Some (tsk (stmt_seq stmt_skip s) l)) q) ->
+      stmt_step σ (<[o:=cn_object C a (Some (tsk s l)) q]> σ)
 
-| step_return: forall Cs σ o a C l e v q f fi,
-    eval Fs (union a l) e v ->
-    σ !! fi = Some (cn_future f None) ->
-    σ !! o = Some (cn_object C a (Some (tsk (stmt_ret e) l)) q) ->
-    l !! destiny = Some (t_fut fi) ->
-    stmt_step Fs Cs σ (<[o:=cn_object C a None q]>
-                      (<[fi:=cn_future f (Some v)]> σ))
+  | step_skip2: forall σ o a C l q,
+      σ !! o = Some (cn_object C a (Some (tsk stmt_skip l)) q) ->
+      stmt_step σ (<[o:=cn_object C a None q]> σ)
 
-| step_read: forall Cs σ o a C l x s v q f fi,
-    σ !! fi = Some (cn_future f (Some v)) ->
-    σ !! o = Some (cn_object C a (Some (tsk (stmt_seq (stmt_asgn x (rhs_get f)) s) l)) q) ->
-    stmt_step Fs Cs σ (<[o:=cn_object C a (Some (tsk (stmt_seq (stmt_asgn x (rhs_e (e_t v))) s) l)) q]> σ)
+  | step_while: forall σ o a C l e s1 s2 q,
+      σ !! o = Some (cn_object C a (Some (tsk (stmt_seq (stmt_loop e s1) s2) l)) q) ->
+      stmt_step σ (<[o:=cn_object C a (Some ( tsk (stmt_seq (stmt_cond e (stmt_seq s1 (stmt_loop e s1)) stmt_skip) s2) l)) q]> σ)
 
-| step_load: forall σ o oi i a p p' q f m vs C CL Cs Cs',
-    σ !! oi = Some (cn_object C a p q) ->
-    σ !! i = Some (cn_invoc o f m vs) ->
-    get_class_name CL = C ->
-    bind m vs f CL = Some p' ->
-    stmt_step Fs (Cs ++ [CL] ++ Cs') σ
-    (<[oi:=cn_object C a p (add p' q)]>
-       (delete i σ))
-.
+  | step_call: forall σ oi o' a C l q x m es vs s f i,
+      fresh f σ ->
+      ~ i ∈ dom σ ->
+      eval_list (union a l) es vs ->
+      σ !! oi = Some (cn_object C a (Some (tsk (stmt_seq (stmt_asgn x (rhs_invoc o' m es)) s) l)) q) ->
+      stmt_step σ (<[oi:=cn_object C a (Some (tsk (stmt_seq (stmt_asgn x (rhs_get f)) s) l)) q]>
+                     (<[i:=cn_invoc o' f m vs]>
+                        (<[id_of f:=cn_future f None]> σ)))
 
-(** Typing *)
+  | step_return: forall σ o a C l e v q f fi,
+      eval (union a l) e v ->
+      σ !! fi = Some (cn_future f None) ->
+      σ !! o = Some (cn_object C a (Some (tsk (stmt_ret e) l)) q) ->
+      l !! destiny = Some (t_fut fi) ->
+      stmt_step σ (<[o:=cn_object C a None q]>
+                     (<[fi:=cn_future f (Some v)]> σ))
+
+  | step_read: forall σ o a C l x s v q f fi,
+      σ !! fi = Some (cn_future f (Some v)) ->
+      σ !! o = Some (cn_object C a (Some (tsk (stmt_seq (stmt_asgn x (rhs_get f)) s) l)) q) ->
+      stmt_step σ (<[o:=cn_object C a (Some (tsk (stmt_seq (stmt_asgn x (rhs_e (e_t v))) s) l)) q]> σ)
+
+  | step_load: forall σ o oi i a p p' q f m vs C CL,
+      σ !! oi = Some (cn_object C a p q) ->
+      σ !! i = Some (cn_invoc o f m vs) ->
+      CL ∈ Cs ->
+      get_class_name CL = C ->
+      bind m vs f CL = Some p' ->
+      stmt_step σ (<[oi:=cn_object C a p (add p' q)]> (delete i σ))
+  .
+End Semantics.
+
+Section Typing.
 (* based on https://link.springer.com/chapter/10.1007/978-3-642-25271-6_8 *)
 
-Inductive typ_method: list CL -> G -> C -> m -> list e -> T -> Prop :=
-(* TODO: implement this *).
-Inductive typ_CL: G -> CL -> Prop :=
-(* TODO: implement this *).
+  Context
+      (Cs: list CL)
+      (Fs: list F)
+      (name_of: id -> f)
+      (id_of: f -> id)
+      (class_of: o -> C)
+  .
 
-Inductive typ_rhs (Cs: list CL): G -> rhs -> ctxv -> Prop :=
-| typ_rhs_e: forall G e T,
-    typ_e G e T ->
-    typ_rhs Cs G (rhs_e e) (ctxv_T T)
-| typ_rhs_invoc: forall G o m es T,
-    typ_method Cs G o m es T ->
-    typ_rhs Cs G (rhs_invoc o m es) (ctxv_fut T)
-| typ_rhs_get: forall G f T,
-    G !! f = Some (ctxv_fut T) ->
-    typ_rhs Cs G (rhs_get f) (ctxv_T T)
-.
+  Hypothesis (vars_fs_distinct: forall (x_:x) (fn:fc), x_ <> fn).
 
-Inductive typ_stmt (Cs: list CL): G -> stmt -> Prop :=
-| typ_stmt_seq: forall G s1 s2,
-    typ_stmt Cs G s1 ->
-    typ_stmt Cs G s2 ->
-    typ_stmt Cs G (stmt_seq s1 s2)
+  Equations typ_es: G -> list e -> list T -> Prop := {
+      typ_es _ [] [] := True ;
+      typ_es Γ (e::es) (T::Ts) := typ_e Γ e T /\ typ_es Γ es Ts ;
+      typ_es _ _ _ := False
+    }.
 
-| typ_stmt_skip: forall G,
-    typ_stmt Cs G stmt_skip
+  Lemma type_preservation_eval: forall Γ,
+      Forall (typ_F Γ) Fs ->
+      forall σ, G_vdash_s Γ σ ->
+           forall e0 e1 T0,
+             typ_e Γ e0 T0 ->
+             eval Fs σ e0 e1 ->
+             typ_e Γ (e_t e1) T0.
+  Proof.
+    intros.
+    destruct H2 as [σ' COMP].
+    pose proof type_preservation vars_fs_distinct  _ _ _ H0 H _ _ _ H1 COMP
+      as (Γ' & SUB & VDASH & TYP).
+    now inv TYP; constructor.
+  Qed.
 
-|typ_stmt_asgn: forall G x r T,
-    G !! x = Some T ->
-    typ_rhs Cs G r T ->
-    typ_stmt Cs G (stmt_asgn x r)
+  Lemma type_preservation_eval_list: forall Γ,
+      Forall (typ_F Γ) Fs ->
+      forall σ, G_vdash_s Γ σ ->
+        forall es vs Ts,
+          typ_es Γ es Ts ->
+          eval_list Fs σ es vs ->
+          typ_es Γ (map e_t vs) Ts.
+  Proof.
+    induction es; intros;
+      destruct vs;
+      destruct Ts;
+      cbn;
+      autorewrite with typ_es eval_list in *;
+      try intuition.
+    eapply type_preservation_eval; eauto.
+  Qed.
 
-| typ_stmt_cond: forall G b s1 s2,
-    typ_e G b T_bool ->
-    typ_stmt Cs G s1 ->
-    typ_stmt Cs G s2 ->
-    typ_stmt Cs G (stmt_cond b s1 s2)
+  Definition add_G (Γ:G) (Tx:T*x): G := <[Tx.2:=ctxv_T Tx.1]> Γ.
+  Definition extend_G (Γ:G) (l:list (T*x)): G := foldr (flip add_G) Γ l.
 
-| typ_stmt_loop: forall G b s,
-    typ_e G b T_bool ->
-    typ_stmt Cs G s ->
-    typ_stmt Cs G (stmt_loop b s)
+  Variant match_method: m -> list T -> T -> CL -> Prop :=
+    match_intro: forall m method Cl,
+        get_method_decl m (get_methods Cl) = Some method ->
+        match_method m (map fst (get_params method)) (get_type method) Cl.
 
-| typ_stmt_return: forall G e T,
-    typ_e G e T ->
-    G !! destiny = Some (ctxv_fut T) ->
-    typ_stmt Cs G (stmt_ret e)
-.
+  Variant typ_rhs: G -> rhs -> ctxv -> Prop :=
+    | typ_rhs_e: forall Γ e T,
+        typ_e Γ e T ->
+        typ_rhs Γ (rhs_e e) (ctxv_T T)
+    | typ_rhs_invoc: forall Γ m o es Cl Ts T,
+        typ_es Γ es Ts ->
+        get_class_decl (class_of o) Cs = Some Cl ->
+        match_method m Ts T Cl ->
+        typ_rhs Γ (rhs_invoc o m es) (ctxv_fut T)
+    | typ_rhs_fut: forall Γ f T,
+        Γ !! f = Some (ctxv_fut T) ->
+        typ_rhs Γ (rhs_get f) (ctxv_T T)
+  .
 
-Definition class_of: o -> C.
-Admitted.
+  Inductive stmt_well_typed: G -> stmt -> Prop :=
+  | typ_stmt_seq: forall G s1 s2,
+      stmt_well_typed G s1 ->
+      stmt_well_typed G s2 ->
+      stmt_well_typed G (stmt_seq s1 s2)
 
-Equations task_well_typed (Cs: list CL) (G0:G) (t:task): Prop := {
-  task_well_typed Cs G0 (tsk p l) := G_vdash_s G0 l /\ typ_stmt Cs G0 p
-  }.
-(* this is a bit weird: the paper treats l sometimes as a list of typed variable bindings and sometimes as local state :/
- if variable bindings then the typ_stmt judgement here should bind those vars in G0 *)
+  | stmt_well_typed_skip: forall G,
+      stmt_well_typed G stmt_skip
 
-Definition queue_well_typed (Cs: list CL) (G0:G) (q:queue): Prop :=
-  forall t, t ∈ q -> task_well_typed Cs G0 t.
+  | stmt_well_typed_asgn: forall G x r T,
+      G !! x = Some T ->
+      typ_rhs G r T ->
+      stmt_well_typed G (stmt_asgn x r)
 
-Inductive cn_well_typed (Cs: list CL): G -> cn -> Prop :=
-| wt_future_none: forall G f T,
-    G !! f = Some (ctxv_fut T) ->
-    cn_well_typed Cs G (cn_future f None)
+  | stmt_well_typed_cond: forall G b s1 s2,
+      typ_e G b T_bool ->
+      stmt_well_typed G s1 ->
+      stmt_well_typed G s2 ->
+      stmt_well_typed G (stmt_cond b s1 s2)
 
-| wt_future_some: forall G f t T,
-    G !! f = Some (ctxv_fut T) ->
-    typ_e G (e_t t) T ->
-    cn_well_typed Cs G (cn_future f (Some t))
+  | stmt_well_typed_loop: forall G b s,
+      typ_e G b T_bool ->
+      stmt_well_typed G s ->
+      stmt_well_typed G (stmt_loop b s)
 
-| wt_invoc: forall G o f m vs T,
-    typ_method Cs G (class_of o) m (map e_t vs) T ->
-    G !! f = Some (ctxv_fut T) ->
-    cn_well_typed Cs G (cn_invoc o f m vs)
+  | stmt_well_typed_return: forall G e T,
+      typ_e G e T ->
+      G !! destiny = Some (ctxv_fut T) ->
+      stmt_well_typed G (stmt_ret e)
+  .
 
-| wt_object_none: forall G C a q,
-    queue_well_typed Cs G q ->
-    cn_well_typed Cs G (cn_object C a None q)
+  Variant task_well_typed: G -> option task -> Prop :=
+    | task_wt_idle: forall Γ, task_well_typed Γ None
+    | task_wt: forall Γ stmt l,
+        (* this differs from the paper since we do not treat l as a typed list *)
+        G_vdash_s Γ l ->
+        stmt_well_typed Γ stmt ->
+        task_well_typed Γ (Some (tsk stmt l))
+  .
 
-| wt_object_some: forall G C a p q,
-    queue_well_typed Cs G q ->
-    task_well_typed Cs G p ->
-    cn_well_typed Cs G (cn_object C a (Some p) q)
-.
+  Definition queue_well_typed (Γ:G) (q:queue) := forall t, t ∈ q -> task_well_typed Γ (Some t).
 
-Definition config_well_typed (Cs: list CL) (G0:G) (conf: config) :=
-  forall i ob, conf !! i = Some ob -> cn_well_typed Cs G0 ob.
+  Variant cn_well_typed: G -> cn -> Prop :=
+    | ob_wt: forall Γ c Cl a p q fields,
+        (* The paper also checks fields(Γ(o)), but we would need another case for ctxv *)
+        get_class_decl c Cs = Some Cl ->
+        get_fields Cl = fields ->
+        queue_well_typed (extend_G Γ fields) q ->
+        task_well_typed (extend_G Γ fields) p ->
+        G_vdash_s (extend_G Γ fields) a ->
+        cn_well_typed Γ (cn_object c a p q)
+    | inv_wt: forall Γ o f T Ts m vs Cl,
+        Γ !! f = Some (ctxv_fut T) ->
+        typ_es Γ (map e_t vs) Ts ->
+        get_class_decl (class_of o) Cs = Some Cl ->
+        match_method m Ts T Cl ->
+        cn_well_typed Γ (cn_invoc o f m vs)
+    | fut_wt_none: forall G f T,
+        G !! f = Some (ctxv_fut T) ->
+        cn_well_typed  G (cn_future f None)
+    | fut_wt_some: forall G f t T,
+        G !! f = Some (ctxv_fut T) ->
+        typ_e G (e_t t) T ->
+        cn_well_typed  G (cn_future f (Some t))
+  .
+  Definition config_well_typed (G0:G) (conf: config) :=
+    forall i ob, conf !! i = Some ob -> cn_well_typed G0 ob.
 
-Theorem type_preservation : forall (Fs: list F) (Cs: list CL) (G0: G),
-    Forall (typ_F G0) Fs ->
-    Forall (typ_CL G0) Cs ->
-    forall σ σ',
-      config_well_typed Cs G0 σ ->
-      stmt_step Fs Cs σ σ' ->
-      exists G',
-        G0 ⊆ G' /\ config_well_typed Cs G' σ'.
-Proof.
-Admitted.
+  (** useful tactics and lemmas *)
 
-(*TODO: subject reduction for stmt_step *)
+  Ltac lookup_cases H i j :=
+    is_eq i j; [setoid_rewrite lookup_insert in H; inv H
+               | setoid_rewrite lookup_insert_ne in H; auto].
+
+  Ltac unfold_typing :=
+    repeat (match goal with
+            | H: cn_well_typed _ _ |- _ => inv H
+            | H: task_well_typed _ _ |- _ => inv H
+            | H: stmt_well_typed _ (stmt_seq _ _) |- _ => inv H
+            | H: stmt_well_typed _ (stmt_asgn _ _) |- _ => inv H
+            | H: stmt_well_typed _ (stmt_cond _ _ _) |- _ => inv H
+            | H: stmt_well_typed _ (stmt_loop _ _) |- _ => inv H
+            | H: stmt_well_typed _ (stmt_ret _) |- _ => inv H
+            | H: typ_rhs _ _ _ |- _ => inv H
+            (* | H: match_method _ _ _ _ |- _ => inv H *)
+            end).
+
+  (* should be a theorem, but will require some assumptions on name_of/id_of and typing of futures *)
+  Hypothesis id_of_consistent: forall (σ:config) f f' v, σ !! (id_of f) = Some (cn_future f' v) -> f = f'.
+  Variant is_fut: cn -> Prop := is_fut_intro: forall f v, is_fut (cn_future f v).
+  Hypothesis id_of_well_typed: forall (σ:config) f c, σ !! (id_of f) = Some c -> is_fut c.
+
+  Lemma fresh_config_wt: forall Γ f σ,
+      fresh f σ -> config_well_typed Γ σ -> f ∉ dom Γ.
+  Proof.
+    unfold fresh, config_well_typed.
+    intros.
+    destruct (σ !! id_of f) eqn:?.
+    - specialize (id_of_well_typed _ _ _ Heqo) as FUT_WT; auto.
+      inv FUT_WT.
+      specialize (H0 _ _ Heqo).
+      specialize (id_of_consistent _ _ _ _ Heqo).
+      intro.
+      eapply H; eauto.
+    - admit.
+      (* this seems problematic *)
+  Admitted.
+
+  Lemma subG_extend: forall Γ l,
+      Forall (fun '(_, x) => x ∉ dom Γ) l ->
+      Γ ⊆ extend_G Γ l.
+  Proof.
+    induction l; intros; auto.
+    destruct a; simpl in *.
+    inv H.
+    eapply subG_add; auto.
+    simpl.
+    now apply not_elem_of_dom.
+  Qed.
+
+  Lemma q_wt_remove: forall  G0 q,
+      queue_well_typed  G0 q ->
+      forall t, queue_well_typed  G0 (remove t q).
+  Proof.
+    intros*.
+    apply H.
+    multiset_solver.
+  Qed.
+
+  Lemma q_wt_add: forall  G0 q,
+      queue_well_typed  G0 q ->
+      forall t,
+        task_well_typed G0 (Some t) ->
+        queue_well_typed  G0 (add t q).
+  Proof.
+    intros*.
+    apply gmultiset_elem_of_disj_union in H1.
+    destruct H1; auto.
+    now apply gmultiset_elem_of_singleton in H1; subst.
+  Qed.
+
+  Lemma G_vdash_union: forall Γ σ σ',
+      G_vdash_s Γ σ ->
+      (* somewhat surprisingly we do not need σ' because map_union prefers the left*)
+      (* G_vdash_s Γ σ' -> *)
+      G_vdash_s Γ (union σ σ').
+  Proof.
+    intros*.
+    apply H in H0.
+    destruct H0 as (?t & LU & TYP).
+    exists t.
+    split; simp; auto.
+  Qed.
+
+  (* this is a problem: well-typing of tasks is not closed under extensions *)
+  Fact subG_task_wt : exists Γ1 Γ2 t,
+      Γ1 ⊆ Γ2 /\ task_well_typed  Γ1 t /\ ~ task_well_typed  Γ2 t.
+  Proof.
+    exists ∅, (<["x":=ctxv_T T_bool]> ∅), (Some (tsk stmt_skip (<["x":=t_int Z0]> ∅))).
+    splits.
+    - now apply insert_subseteq.
+    - econstructor.
+      + intros*.
+        inv H.
+      + constructor.
+    - inv 1.
+      pose proof H3 "x" (ctxv_T T_bool) as (?t' & ? & ?); auto.
+      simpl in H0.
+      inv H0.
+  Qed.
+
+  (* this substitution and subsequent well-typing is not currently used *)
+  (* I thought I might use it, and then didn't, but may be useful later? *)
+  Equations e_subst_s : s -> e -> e := {
+      e_subst_s _ (e_t t) := e_t t;
+      e_subst_s σ (e_var x_) := match σ !! x_ with | Some t => (e_t t) | None => (e_var x_) end ;
+      e_subst_s σ (e_fn_call fn_ es) := e_fn_call fn_ (e_subst_list_s σ es) }
+  where e_subst_list_s: s -> list e -> list e := {
+      e_subst_list_s _ [] := [] ;
+      e_subst_list_s σ (e_::es) := e_subst_s σ e_ :: e_subst_list_s σ es
+    }.
+
+  (* the well-typedness from the paper, ours is a little stricter *)
+  Definition sub_well_typed (Γ : G) (σ : s) :=
+    forall (x_: x) (T_: T),
+      x_ ∈ dom σ ->
+      Γ !! x_ = Some (ctxv_T T_) ->
+      typ_e Γ (e_subst_s σ (e_var x_)) T_.
+
+  Lemma vdash_implies_wt: forall Γ σ,
+      G_vdash_s Γ σ ->
+      sub_well_typed Γ σ.
+  Proof.
+    intros*.
+    pose proof H x_ (ctxv_T T_) H1 as (?t_ & LU & TYP).
+    autorewrite with e_subst_s.
+    now rewrite LU.
+  Qed.
+
+  (* just like our vdash, this is the wrong way *)
+  Lemma subG_sub_wt: forall Γ1 Γ2 σ,
+      Γ1 ⊆ Γ2 -> sub_well_typed Γ2 σ -> sub_well_typed Γ1 σ.
+  Proof.
+    intros*.
+    specialize (H0 x_ T_ H1).
+    autorewrite with e_subst_s in *.
+    apply elem_of_dom in H1.
+    inv H1.
+    setoid_rewrite H3.
+    eapply map_subseteq_spec in H; eauto.
+    apply H0 in H.
+    setoid_rewrite H3 in H.
+    inv H; constructor.
+  Qed.
+
+  Lemma subG_typ_es: forall G1 G2 es Ts,
+      subseteq G1 G2 -> typ_es G1 es Ts -> typ_es G2 es Ts.
+  Proof.
+    induction es; destruct Ts; auto; intros.
+    autorewrite with typ_es in *.
+    destruct H0.
+    split; auto.
+    eapply subG_type; eauto.
+  Qed.
+
+  Lemma subG_typ_rhs: forall G1 G2 r T0,
+      subseteq G1 G2 -> typ_rhs G1 r T0 -> typ_rhs G2 r T0.
+  Proof.
+    intros.
+    inv H0.
+    - econstructor.
+      eapply subG_type; eauto.
+    - econstructor; eauto.
+      eapply subG_typ_es; eauto.
+    - econstructor.
+      eapply lookup_weaken; eauto.
+  Qed.
+
+  Lemma subG_stmt_wt: forall G1 G2 st,
+      subseteq G1 G2 -> stmt_well_typed G1 st -> stmt_well_typed G2 st.
+  Proof.
+    intros.
+    induction H0; eauto;
+      try (now econstructor; eauto).
+    - econstructor.
+      + eapply lookup_weaken; eauto.
+      + eapply subG_typ_rhs; eauto.
+    - econstructor; eauto.
+      eapply subG_type; eauto.
+    - econstructor; eauto.
+      eapply subG_type; eauto.
+    - econstructor.
+      + eapply subG_type; eauto.
+      + eapply lookup_weaken; eauto.
+  Qed.
+
+  Lemma fresh_extend_wt: forall Γ σ f,
+      config_well_typed Γ σ ->
+      fresh f σ ->
+      forall T_,
+        config_well_typed (<[f:=T_]> Γ) σ.
+  Proof.
+  Admitted.
+
+  Theorem type_preservation : forall (Γ: G),
+      Forall (typ_F Γ) Fs ->
+      forall σ σ',
+        config_well_typed Γ σ ->
+        stmt_step Cs Fs id_of σ σ' ->
+        exists Γ', Γ ⊆ Γ' /\ config_well_typed Γ' σ'.
+  Proof.
+    intros.
+    inv H1.
+    - exists Γ; split; auto.
+      intros*.
+      lookup_cases H1 i i0.
+      + specialize (H0 _ _ H3).
+        unfold_typing.
+        destruct p.
+        econstructor; eauto.
+        now apply q_wt_remove.
+      + eapply H0;eauto.
+
+    - destruct H3 as [sf ?].
+      pose proof H1 as Conf_wt.
+      specialize (H0 _ _ H4).
+      unfold_typing.
+      epose proof type_preservation _ _ _ _ _ _ _ _ _ H5 H1
+        as (?Γ & ?SUB & ? & ?TYP_E).
+      (* are tasks actually well-typed under this extension? *)
+      admit.
+      Unshelve.
+      + apply vars_fs_distinct.
+      + now apply G_vdash_union.
+      + apply subG_typ_F_forall with Γ; auto.
+        apply subG_extend.
+        admit. (* can we guarantee that the fields are not already in the context? *)
+
+    - destruct H3 as [sf ?].
+      pose proof H1 as Conf_wt.
+      specialize (H0 _ _ H4).
+      unfold_typing.
+      epose proof type_preservation _ _ _ _ _ _ _ _ _ H5 H1
+        as (?Γ & ?SUB & ? & ?TYP_E).
+      admit.
+
+    (* the trivial cases (ifs, skips, loops) are very similar*)
+    (* TODO: automate *)
+    - pose proof H0 as Conf_wt.
+      specialize (H0 _ _ H3).
+      unfold_typing.
+      exists Γ; split; auto.
+      intros*.
+      lookup_cases H0 o i.
+      + repeat (econstructor; eauto).
+      + eapply Conf_wt; eauto.
+
+    - pose proof H0 as Conf_wt.
+      specialize (H0 _ _ H3).
+      unfold_typing.
+      exists Γ; split; auto.
+      intros*.
+      lookup_cases H0 o i.
+      + repeat (econstructor; eauto).
+      + eapply Conf_wt; eauto.
+
+    - pose proof H0 as Conf_wt.
+      specialize (H0 _ _ H2).
+      unfold_typing.
+      exists Γ; split; auto.
+      intros*.
+      lookup_cases H0 o i.
+      + repeat (econstructor; eauto).
+      + eapply Conf_wt; eauto.
+
+    - pose proof H0 as Conf_wt.
+      specialize (H0 _ _ H2).
+      unfold_typing.
+      exists Γ; split; auto.
+      intros*.
+      lookup_cases H0 o i.
+      + repeat (econstructor; eauto).
+      + eapply Conf_wt; eauto.
+
+    - pose proof H0 as Conf_wt.
+      specialize (H0 _ _ H2).
+      unfold_typing.
+      exists Γ; split; auto.
+      intros*.
+      lookup_cases H0 o i.
+      + repeat (econstructor; eauto).
+      + eapply Conf_wt; eauto.
+
+    - pose proof H0 as Conf_wt.
+      specialize (H0 _ _ H5).
+      unfold_typing.
+      pose proof H18 as Method_wt.
+      inv H18.
+      destruct method.
+      autorewrite with get_type get_params in *.
+      epose proof type_preservation_eval_list _ _ _ _ _ _ _ H15 H4 as TYP_ARGS.
+      exists (<[f:=ctxv_fut T_5]> Γ).
+      split.
+      + apply subG_add; auto.
+        apply not_elem_of_dom.
+        eapply fresh_config_wt; eauto.
+      + intros*.
+        lookup_cases H1 oi i0.
+        * econstructor; eauto.
+          -- admit.
+          -- constructor; auto.
+             ++ admit.
+             ++ econstructor.
+                ** econstructor; eauto.
+                   --- admit.
+                   --- econstructor.
+                       eapply lookup_weaken with (<[f:=ctxv_fut T_5]> Γ).
+                       +++ apply lookup_insert.
+                       +++ apply subG_extend.
+                           admit.
+                ** eapply subG_stmt_wt.
+                   --- admit.
+                   --- eauto.
+          -- admit. (* should follow from freshness *)
+        * lookup_cases H1 i i0.
+          -- econstructor; eauto.
+             ++ apply lookup_insert.
+             ++ admit. (* I would like to use TYP_ARGS, but that includes the fields from the object *)
+          -- set (fi:=id_of f).
+             is_eq fi i0; subst fi.
+             ++ setoid_rewrite lookup_insert in H1.
+                inv H1.
+                econstructor.
+                apply lookup_insert.
+             ++ setoid_rewrite lookup_insert_ne in H1; auto.
+                eapply fresh_extend_wt; eauto.
+
+    - pose proof H0 _ _ H3 as fut_well_typed.
+      pose proof H0 _ _ H4 as ob_well_typed.
+      exists Γ; split; auto.
+      intros*.
+      unfold_typing.
+      lookup_cases H1 o i.
+      + econstructor; eauto.
+        econstructor.
+      + lookup_cases H1 fi i.
+        * econstructor; eauto.
+          epose proof type_preservation_eval _ _ _ _ _ _ _ H7 H2.
+          enough (T0 = T) by (subst; inv H1; constructor).
+          pose proof (H11 _ _ H14) as (?t & ? & ?); simp.
+          inv H1; inv H9.
+        * eapply H0; eauto.
+
+    - pose proof H0 _ _ H2 as fut_well_typed.
+      pose proof H0 _ _ H3 as ob_well_typed.
+      exists Γ; split; auto.
+      intros*.
+      unfold_typing.
+      lookup_cases H1 o i.
+      + repeat (econstructor; eauto).
+        replace T1 with T by admit. (* follows from f ∉ fields(Cl) *)
+        eapply subG_type with Γ; auto.
+        apply subG_extend.
+        admit.
+      + eapply H0; eauto.
+
+    - pose proof H0 _ _ H2 as ob_well_typed.
+      pose proof H0 _ _ H3 as inv_well_typed.
+      exists Γ; split; auto.
+      intros*.
+      unfold_typing.
+      + lookup_cases H1 oi i0.
+        * repeat (econstructor; eauto).
+          apply q_wt_add; auto.
+          admit. (* here we need Γ ⊢ Cl -> Γ ⊢ bind m vs f*)
+        * is_eq i i0.
+          -- exfalso.
+             setoid_rewrite (lookup_delete σ i) in H1.
+             inv H1.
+          -- setoid_rewrite lookup_delete_ne in H1; auto.
+             eapply H0; eauto.
+      + lookup_cases H1 oi i0.
+        * repeat (econstructor; eauto).
+          apply q_wt_add; auto.
+          admit. (* here we need Γ ⊢ Cl -> Γ ⊢ bind m vs f*)
+        * is_eq i i0.
+          -- exfalso.
+             setoid_rewrite (lookup_delete σ i) in H1.
+             inv H1.
+          -- setoid_rewrite lookup_delete_ne in H1; auto.
+             eapply H0; eauto.
+
+             Unshelve.
+             all: try eauto.
+             all: try (now apply G_vdash_union).
+             (*remaining: typ_F closed under (well-typed?) extensions *)
+  Admitted.
+End Typing.
 (*TODO: labels + traces? *)
